finished the proof of neutral property.

QVM/PQASM.v
@@ -4115,18 +4115,6 @@ Fixpoint avars (l: list (var * nat)) (dim:nat) : (nat -> posi) :=
                                        else avars l' (dim + n) i
     end.
        
-(*                                                                            
-Lemma vs_bij : forall l dim vs avs, dim = get_dim l ->
-            vs = compile_var' l 0 -> vars_WF l -> avs = avars l 0 ->
-         (forall x y, y < vsize vs x -> 
-              (forall i, i < dim -> avs (find_pos vs (x,y)) = (x,y))).
-Proof.
-  intros. subst.
-  induction l. simpl in H5. lia.
-  simpl.
-  destruct a eqn:eq1.
-Admitted.
-*)
 
 Lemma compile_var'_WF : forall l dim p vs, vs = compile_var' l dim
               -> snd p < vsize vs (fst p) -> find_pos vs p < dim + get_dim l.
@@ -6339,38 +6327,1224 @@ Proof.
   intros R. inv R. specialize (IHl a0). contradiction.
 Qed.
 
-Lemma neu_l_trans_state : forall e x l vs dim avs, exp_neu_l x l e l -> snd (fst (trans_exp vs dim e avs)) x = vs x.
+(* Define two properties for neu. First, we show that for every x exp_neu_l l l',
+        l' is either a subsequence of l or l is a subsequence of l'. 
+   The secord property relates l l' with avs and avs', so
+   for every exp_neu_l l l', if l is lated to avs then l' is also linked to avs' in someway. *)
+Fixpoint cut_n_list {A} (n:nat) (l : list A) :=
+   match n with 0 => Some l
+             | S m => match l with [] => None
+                                 | (a::al) => cut_n_list m al
+                      end
+   end.
+
+Fixpoint get_n_list {A} (n:nat) (l : list A) :=
+   match n with 0 => Some ([])
+        | S m => match l with [] => None
+                            | (a::al) => match get_n_list m al with None => None
+                                                                  | Some l' => Some (a::l')
+                                         end
+                  end
+    end.
+
+Lemma cut_n_list_0 {A:Type} : forall (l:list A), cut_n_list 0 l = Some l.
 Proof.
-  induction e; intros; try easy.
-  simpl. destruct (trans_exp vs dim e avs). destruct p0.
-  simpl. easy.
-  inv H0. apply list_neq in H2. inv H2.
-  assert (l = Ls :: l) by easy.
-  apply list_neq in H0. inv H0.
-  simpl.
-  unfold trans_lshift.
-  destruct (vs x). destruct p. destruct p.
-  bdestruct (x0 =? x). lia.
-  easy.
-  inv H0. apply list_neq in H2. inv H2.
-  assert (l = Rs :: l) by easy.
-  apply list_neq in H0. inv H0.
-  simpl.
-  unfold trans_rshift.
-  destruct (vs x). destruct p. destruct p.
-  bdestruct (x0 =? x). lia.
-  easy.
-  inv H0. apply list_neq in H2. inv H2.
-  assert (l = Re :: l) by easy.
-  apply list_neq in H0. inv H0.
-  simpl.
-  unfold trans_rev.
-  destruct (vs x). destruct p. destruct p.
-  bdestruct (x0 =? x). lia.
-  easy.
-  inv H0.
+ intros. simpl in *. easy.
+Qed.
+
+Lemma get_cut_n_list_same {A:Type} : forall n (l l1 l2: list A), cut_n_list n l = Some l1
+           -> get_n_list n l = Some l2 -> (l2 ++ l1) = l.
+Proof.
+  induction n; intros; simpl in *.
+  inv H0. inv H1. easy.
+  destruct l. inv H0.
+  destruct (get_n_list n l) eqn:eq1.
+  inv H1.
+  specialize (IHn l l1 l0 H0 eq1).
+  rewrite <- IHn. easy. inv H1.
+Qed.
+
+Lemma get_n_list_empty {A:Type}: forall n (l: list A), get_n_list n l = Some ([]) -> n = 0.
+Proof.
+  induction n; intros; simpl in *. easy.
+  destruct l. inv H0.
+  destruct (get_n_list n l) eqn:eq1. inv H0. inv H0.
+Qed.
+
+Lemma get_cut_n_list_same_1 {A:Type} : forall n (l l1: list A), cut_n_list n l = Some l
+   -> get_n_list n l = Some l1 -> n = 0.
+Proof.
+  intros.
+  specialize (get_cut_n_list_same n l l l1 H0) as eq1.
+  apply eq1 in H1 as eq2.
+  assert (l = ([])++l).
+  rewrite app_nil_l. easy.
+  assert (l1 ++ l = [] ++ l).
+  rewrite eq2. easy.
+  apply app_inv_tail in H3. subst.
+  apply get_n_list_empty in H1. easy.
+Qed.
+
+Lemma cut_n_list_add {A:Type} : forall n n1 (l l1 l2: list A),
+       cut_n_list n l = Some l1 -> cut_n_list n1 l1 = Some l2 -> cut_n_list (n + n1) l = Some l2.
+Proof.
+  induction n; intros;simpl.
+  rewrite cut_n_list_0 in H0. inv H0. easy.
+  simpl in *. destruct l. inv H0.
+  rewrite IHn with (l1 := l1) (l2 := l2); try easy.
+Qed.
+
+Lemma cut_n_list_sub {A:Type} : forall n n1 (l l1 l2: list A), n <= n1 ->
+       cut_n_list n l = Some l1 -> cut_n_list n1 l = Some l2 -> cut_n_list (n1-n) l1 = Some l2.
+Proof.
+  induction n; intros;simpl.
+  rewrite cut_n_list_0 in H1. inv H1.
+  assert ((n1 - 0) = n1) by lia. rewrite H1. easy.
+  destruct n1. lia. simpl in H1. simpl in H2.
+  destruct l. inv H1.
+  assert (n <= n1) by lia.
+  specialize (IHn n1 l l1 l2 H3 H1 H2).
+  assert (S n1 - S n = n1 - n) by lia. rewrite H4. easy.
+Qed.
+
+Definition exp_neu_sub_prop (l l' : list sexp) :=
+       (exists n, cut_n_list n l' = Some l \/ cut_n_list n l = Some l').
+
+Lemma exp_neu_sub_keep : forall e x l l', exp_neu_l x l e l' -> exp_neu_sub_prop l l'.
+Proof.
+  intros. unfold exp_neu_sub_prop. induction H0.
+  exists 0. left. apply cut_n_list_0.
+  exists 0. left. apply cut_n_list_0.
+  exists 0. left. apply cut_n_list_0.
+  exists 0. left. apply cut_n_list_0.
+  exists 0. left. apply cut_n_list_0.
+  exists 0. left. apply cut_n_list_0.
+  exists 0. left. apply cut_n_list_0.
+  exists 0. left. apply cut_n_list_0.
+  exists 0. left. apply cut_n_list_0.
+  exists 0. left. apply cut_n_list_0.
+  exists 0. left. apply cut_n_list_0.
+  exists 1. right. simpl in *. easy.
+  exists 1. left. simpl in *. easy.
+  exists 0. left. apply cut_n_list_0.
+  exists 1. right. simpl in *. easy.
+  exists 1. left. simpl in *. easy.
+  exists 0. left. apply cut_n_list_0.
+  exists 1. right. simpl in *. easy.
+  exists 1. left. simpl in *. easy.
+  exists 0. left. apply cut_n_list_0.
+  destruct IHexp_neu_l1. destruct H0.
+  destruct IHexp_neu_l2. destruct H1.
+  exists (x1 + x0). left.
+  apply cut_n_list_add with (l1 := l'); try easy.
+  bdestruct (x0 <=? x1).
+  Check cut_n_list_sub.
+  specialize (cut_n_list_sub x0 x1 l' l l'' H2 H0 H1) as eq1.
+  exists (x1 - x0). right. easy.
+  assert (x1 <= x0) by lia.
+  specialize (cut_n_list_sub x1 x0 l' l'' l H3 H1 H0) as eq1.
+  exists (x0 - x1). left. easy.
+  destruct IHexp_neu_l2.
+  destruct H1. admit.
+  exists (x0 + x1).
+  right. apply cut_n_list_add with (l1 := l'); try easy.
 Admitted.
 
+Definition inter_neu_elem (s:sexp) (f:vars) (x:var) :=
+   match s with Ls => trans_lshift f x
+              | Rs => trans_rshift f x
+              | Re => trans_rev f x
+   end.
+
+
+Fixpoint inter_neu_l (l :list sexp) (f:vars) (x:var) :=
+    match l with [] => f
+            | (a::al) => inter_neu_elem a (inter_neu_l al f x) x
+    end.
+
+Definition inter_neu_elem_anti (s:sexp) (f:vars) (x:var) :=
+   match s with Ls => trans_rshift f x
+              | Rs => trans_lshift f x
+              | Re => trans_rev f x
+   end.
+
+
+Fixpoint inter_neu_l_anti (l :list sexp) (f:vars) (x:var) :=
+    match l with [] => f
+            | (a::al) => (inter_neu_l_anti al (inter_neu_elem_anti a f x) x)
+    end.
+
+Definition exp_neu_trans_prop (x:var) (l l' : list sexp) (vs vs' : vars) :=
+     if length l <=? length l' then 
+       (forall n l1, cut_n_list n l' = Some l -> get_n_list n l' = Some l1 -> vs' x = (inter_neu_l l1 vs x) x)
+    else (forall n l1, cut_n_list n l = Some l' -> get_n_list n l = Some l1 -> vs' x = (inter_neu_l_anti l1 vs x) x).
+
+Lemma cut_n_l_le {A:Type} : forall n (l:list A), n <= length l -> cut_n_list n l <> None.
+Proof.
+  induction n; intros; simpl in *.
+  easy.
+  destruct l. simpl in *. lia.
+  simpl in *.
+  apply IHn. lia.
+Qed.
+
+Lemma length_gt_cut_l {A:Type}: forall (l l' : list A) n, length l <= length l' -> n <= length l' - length l -> 
+                (cut_n_list n l' <> None).
+Proof.
+  induction l;intros;simpl in *.
+  apply cut_n_l_le. lia.
+  apply IHl. lia. lia.
+Qed.
+
+Lemma cut_l_length_le {A:Type}: forall n (l l' : list A), (cut_n_list n l = Some l') -> length l' <= length l.
+Proof.
+  induction n; intros; simpl in *.
+  inv H0. easy.
+  destruct l. easy. specialize (IHn l l' H0). simpl in *. lia.
+Qed.
+
+Lemma get_n_l_le {A:Type} : forall n (l:list A), n <= length l -> get_n_list n l <> None.
+Proof.
+  induction n; intros; simpl in *.
+  easy.
+  destruct l. simpl in *. lia.
+  simpl in *.
+  destruct (get_n_list n l) eqn:eq1. easy.
+  assert (n <= length l) by lia. apply IHn in H1. easy.
+Qed.
+
+Lemma cut_n_length_le {A:Type} : forall n (l:list A), cut_n_list n l <> None -> n <= length l.
+Proof.
+  induction n; intros; simpl in *.
+  lia.
+  destruct l. easy.
+  apply IHn in H0. simpl. lia.
+Qed.
+
+Lemma get_n_list_not_none {A:Type}: forall n (l : list A),
+ get_n_list n l <> None -> (exists (l1:list A), get_n_list n l = Some l1).
+Proof.
+  induction n; intros; simpl in *. exists nil. easy.
+  destruct l. easy.  destruct (get_n_list n l) eqn:eq1.
+  exists (a :: l0). easy.
+  easy.
+Qed.
+
+
+Lemma get_cut_n_list_same_2 {A:Type} : forall n (l: list A), cut_n_list n l = Some l
+   -> get_n_list n l = Some ([]).
+Proof.
+  intros.
+  assert (n <= length l). apply cut_n_length_le. rewrite H0. easy.
+  apply get_n_l_le in H1.
+  apply get_n_list_not_none in H1. destruct H1.
+  specialize (get_cut_n_list_same n l l x H0 H1) as eq1.
+  assert (l = ([])++l).
+  rewrite app_nil_l. easy.
+  assert (x ++ l = [] ++ l).
+  rewrite eq1. easy.
+  apply app_inv_tail in H3. subst. easy.
+Qed.
+
+Lemma list_sub_neq  {A:Type} : forall a (l:list A), (a::l) <> l.
+Proof.
+  intros. induction l;simpl. easy.
+  intros R. inv R. easy.
+Qed.
+
+Lemma get_cut_n_list_1_aux {A:Type} : forall n (a:A) (l : list A), 1 < n -> cut_n_list n (a::l) <> Some l.
+Proof.
+  induction n; intros; simpl. lia.
+  destruct n. lia. destruct n.
+  simpl. destruct l. easy. intros R. inv R.
+  assert (a0 :: l = l) by easy.
+  apply list_sub_neq in H1. easy.
+  assert (1 < S (S n)) by lia.
+  apply (IHn a l) in H1. simpl in *.
+  destruct l. easy. destruct l. easy.
+  intros R.
+  apply cut_l_length_le in R as eq1. simpl in *. lia.
+Qed.
+
+Lemma get_cut_n_list_1 {A:Type} : forall n (a:A) (l : list A), cut_n_list n (a::l) = Some l -> n = 1.
+Proof.
+  intros. destruct n. simpl in *. inv H0.
+  apply list_sub_neq in H2. easy.
+  bdestruct (S n =? 1). easy.
+  assert (1 < S n) by lia.
+  apply (get_cut_n_list_1_aux (S n) a l) in H2. easy.
+Qed.
+
+Lemma get_cut_n_list_n {A:Type} : forall n (l l' : list A), cut_n_list n l' = Some l -> n = length l' - length l.
+Proof.
+  induction n; intros; simpl in *.
+  inv H0. lia.
+  destruct l'. inv H0. apply cut_l_length_le in H0 as X1.
+  apply IHn in H0. simpl. destruct (length l) eqn:eq1. rewrite H0. lia.
+  rewrite H0. simpl. lia.
+Qed.
+
+Lemma cut_get_l_exists {A:Type} : forall n (l l' : list A), cut_n_list n l' = Some l -> (exists l1, get_n_list n l' = Some l1).
+Proof.
+  induction n;intros;simpl in *.
+  exists ([]). easy.
+  destruct l'. inv H0.
+  apply IHn in H0. destruct H0.
+  rewrite H0.
+  exists (a :: x). easy.
+Qed.
+
+Lemma inter_neu_l_assoc : forall (l2 l1 l: list sexp) (vs vs1 vs2:vars) (x:var),
+       l = l2++l1 -> inter_neu_l l1 vs x x = vs1 x -> inter_neu_l l2 vs1 x x = vs2 x
+         -> inter_neu_l l vs x x = vs2 x.
+Proof.
+  induction l2; intros; simpl in *.
+  subst. rewrite H1. easy.
+  remember ((inter_neu_l l2 vs1 x)) as vs'.
+  rewrite H0. simpl.
+  specialize (IHl2 l1 (l2 ++ l1) vs vs1 vs' x).
+  apply IHl2 in H1; try easy.
+  rewrite <- H2.
+  destruct a.
+  simpl.
+  unfold trans_lshift.
+  rewrite H1.
+  destruct (vs' x) eqn:eq1. destruct p. destruct p.
+  bdestruct (x =? x). easy. lia.
+  simpl.
+  unfold trans_rshift.
+  rewrite H1.
+  destruct (vs' x) eqn:eq1. destruct p. destruct p.
+  bdestruct (x =? x). easy. lia.
+  simpl.
+  unfold trans_rev.
+  rewrite H1.
+  destruct (vs' x) eqn:eq1. destruct p. destruct p.
+  bdestruct (x =? x). easy. lia.
+  rewrite Heqvs'. easy.
+  Qed.
+
+Lemma shift_fun_twice_same : forall f size, shift_fun (shift_fun f (size-1) size) 1 size = f.
+Proof.
+  intros. unfold shift_fun.
+  apply functional_extensionality. intros.
+  bdestruct (x <? size).
+  assert (0 < size) by lia.
+  bdestruct ((x + 1) mod size <? size).
+  assert (x+1 <= size) by lia.
+  bdestruct (x + 1 =? size).
+  rewrite H4.
+  rewrite Nat.mod_same by lia.
+  rewrite plus_0_l.
+  rewrite Nat.mod_small by lia.
+  assert (x = size-1) by lia.
+  rewrite H5. easy.
+  assert (x + 1 < size) by lia.
+  rewrite Nat.mod_small with (a := (x + 1)) by lia.
+  assert (((x + 1 + (size - 1)) = x + size)) by lia.
+  rewrite H6.
+  rewrite Nat.add_mod by lia.
+  rewrite Nat.mod_same by lia. rewrite plus_0_r.
+  rewrite Nat.mod_mod by lia.
+  rewrite Nat.mod_small by lia. easy.
+  assert ((x + 1) mod size < size).
+  apply Nat.mod_upper_bound. lia.
+  lia. easy.
+Qed.
+
+Lemma shift_fun_twice_same_1 : forall f size, shift_fun (shift_fun f 1 size) (size-1) size = f.
+Proof.
+  intros. unfold shift_fun.
+  apply functional_extensionality. intros.
+  bdestruct (x <? size).
+  assert (0 < size) by lia.
+  bdestruct ((x + (size - 1)) mod size <? size).
+  rewrite Nat.add_mod by lia.
+  bdestruct (size =? 1). subst.
+  rewrite Nat.mod_same by lia. rewrite plus_0_r.
+  assert ((x + (1 - 1)) = x) by lia. rewrite H3.
+  repeat rewrite Nat.mod_mod by lia.
+  rewrite Nat.mod_small by lia. easy.
+  rewrite Nat.mod_mod by lia.
+  rewrite <- Nat.add_mod by lia.
+  assert ((x + (size - 1) + 1) = x + size) by lia.
+  rewrite H4.
+  rewrite Nat.add_mod by lia.
+  rewrite Nat.mod_same by lia. rewrite plus_0_r.
+  rewrite Nat.mod_mod by lia.
+  rewrite Nat.mod_small by lia. easy.
+  assert ((x + (size - 1)) mod size < size).
+  apply Nat.mod_upper_bound ; lia. lia. easy.
+Qed.
+
+Lemma ashift_fun_twice_same : forall f size,
+    (forall i, i < size -> f i < size) ->
+    ashift_fun (ashift_fun f 1 size) (size-1) size = f.
+Proof.
+  intros. unfold ashift_fun.
+  apply functional_extensionality. intros.
+  bdestruct (x <? size).
+  assert (0 < size) by lia.
+  assert (f x < size). apply H0. easy.
+  bdestruct (f x + 1 =? size).
+  rewrite H4.
+  rewrite Nat.mod_same by lia.
+  rewrite plus_0_l.
+  rewrite Nat.mod_small by lia.
+  rewrite <- H4. lia.
+  assert (f x + 1 < size) by lia.
+  rewrite Nat.mod_small with (a := (f x + 1)) by lia.
+  assert (((f x + 1 + (size - 1)) = f x + size)) by lia.
+  rewrite H6.
+  rewrite Nat.add_mod by lia.
+  rewrite Nat.mod_same by lia. rewrite plus_0_r.
+  rewrite Nat.mod_mod by lia.
+  rewrite Nat.mod_small by lia. easy.
+  easy.
+Qed.
+
+Lemma ashift_fun_twice_same_1 : forall f size,
+    (forall i, i < size -> f i < size) ->
+    ashift_fun (ashift_fun f (size-1) size) 1 size = f.
+Proof.
+  intros. unfold ashift_fun.
+  apply functional_extensionality. intros.
+  bdestruct (x <? size).
+  assert (0 < size) by lia.
+  assert (f x < size). apply H0. easy.
+  rewrite Nat.add_mod by lia.
+  bdestruct (size =? 1). subst.
+  rewrite Nat.mod_same by lia.
+  rewrite plus_0_r.
+  rewrite Nat.mod_mod by lia.
+  rewrite Nat.mod_mod by lia.
+  assert (1-1 = 0) by lia. rewrite H4.
+  rewrite plus_0_r.
+  rewrite Nat.mod_small by lia. easy. 
+  rewrite Nat.mod_small with (a := ((f x + (size - 1)) mod size)).
+  rewrite <- Nat.add_mod by lia.
+  assert ((f x + (size - 1) + 1) = f x + size) by lia.
+  rewrite H5.
+  rewrite Nat.add_mod by lia.
+  rewrite Nat.mod_small with (a := f x) by lia.
+  rewrite Nat.mod_same by lia.
+  rewrite plus_0_r.
+  rewrite Nat.mod_small by lia. easy.
+  apply Nat.mod_upper_bound. lia. easy.
+Qed.
+
+Lemma inter_neu_l_vars_anti_same : 
+   forall l vs x, vars_anti_same vs -> vars_anti_same (inter_neu_l l vs x).
+Proof.
+  induction l;intros;simpl in *. easy.
+  destruct a. simpl.
+  specialize (vars_anti_vs_same (Lshift x) 0 (inter_neu_l l vs x) (snd
+       (fst
+          (trans_exp (inter_neu_l l vs x) 0 
+             (Lshift x) (fun _ : nat => (0, 0))))) (fun _ => (0,0))) as eq1.
+  apply eq1. easy. apply IHl. easy.
+  simpl.
+  specialize (vars_anti_vs_same (Rshift x) 0 (inter_neu_l l vs x) (snd
+       (fst
+          (trans_exp (inter_neu_l l vs x) 0 
+             (Rshift x) (fun _ : nat => (0, 0))))) (fun _ => (0,0))) as eq1.
+  apply eq1. easy. apply IHl. easy.
+  simpl.
+  specialize (vars_anti_vs_same (Rev x) 0 (inter_neu_l l vs x) (snd
+       (fst
+          (trans_exp (inter_neu_l l vs x) 0 
+             (Rev x) (fun _ : nat => (0, 0))))) (fun _ => (0,0))) as eq1.
+  apply eq1. easy. apply IHl. easy.
+Qed.
+
+Lemma afbrev_twice_same: forall size f,
+      (forall i, i < size -> f i < size) ->
+       afbrev (afbrev f size) size = f.
+Proof.
+  intros.
+  unfold afbrev.
+  apply functional_extensionality.
+  intros.
+  bdestruct (x <? size).
+  assert (f x < size). apply H0. easy.
+  assert (0 < size) by lia.
+  assert (f x <= size - 1) by lia.
+  assert (size - 1 - (size - 1 - f x) = f x) by lia.
+  rewrite H5. easy. easy.
+Qed.
+
+Lemma inter_neu_l_rev_same : forall (l: list sexp) vs vs1 x, inter_neu_l l vs x x = vs1 x ->
+       vars_anti_same vs -> inter_neu_l_anti l vs1 x x = vs x.
+Proof.
+  induction l;intros;simpl in *. easy.
+  assert (vars_anti_same (inter_neu_l l vs x)) as eq1. apply inter_neu_l_vars_anti_same. easy.
+  destruct a. simpl in *.
+  specialize (IHl vs (trans_rshift vs1 x) x).
+  rewrite <- IHl. easy.
+  unfold trans_rshift in *. rewrite <- H0.
+  unfold trans_lshift.
+  destruct (inter_neu_l l vs x x) eqn:eq2. destruct p. destruct p.
+  bdestruct (x =? x).
+  bdestruct (x =? x).
+  rewrite shift_fun_twice_same.
+  rewrite ashift_fun_twice_same. easy.
+  unfold vars_anti_same in H1.
+  destruct (eq1 x) as [X1 [X2 [X3 [X4 [X5 X6]]]]].
+  intros. specialize (X3 i).
+  unfold vsize,avmap in X3. rewrite eq2 in *. simpl in X3. apply X3. easy.
+  lia. lia. easy.
+  simpl in *.
+  specialize (IHl vs (trans_lshift vs1 x) x).
+  rewrite <- IHl. easy.
+  unfold trans_lshift in *. rewrite <- H0.
+  unfold trans_rshift.
+  destruct (inter_neu_l l vs x x) eqn:eq2. destruct p. destruct p.
+  bdestruct (x =? x).
+  bdestruct (x =? x).
+  rewrite shift_fun_twice_same_1.
+  rewrite ashift_fun_twice_same_1. easy.
+  unfold vars_anti_same in H1.
+  destruct (eq1 x) as [X1 [X2 [X3 [X4 [X5 X6]]]]].
+  intros. specialize (X3 i).
+  unfold vsize,avmap in X3. rewrite eq2 in *. simpl in X3. apply X3. easy.
+  lia. lia. easy.
+  simpl in *.
+  specialize (IHl vs (trans_rev vs1 x) x).
+  rewrite <- IHl. easy.
+  unfold trans_rev in *. rewrite <- H0.
+  destruct (inter_neu_l l vs x x) eqn:eq2. destruct p. destruct p.
+  bdestruct (x =? x).
+  bdestruct (x =? x).
+  rewrite fbrev_twice_same.
+  rewrite afbrev_twice_same. easy.
+  unfold vars_anti_same in H1.
+  destruct (eq1 x) as [X1 [X2 [X3 [X4 [X5 X6]]]]].
+  intros. specialize (X3 i).
+  unfold vsize,avmap in X3. rewrite eq2 in *. simpl in X3. apply X3. easy.
+  lia. lia. easy.
+Qed.
+
+Lemma inter_neu_anti_vars_anti_same : 
+   forall l vs x, vars_anti_same vs -> vars_anti_same (inter_neu_l_anti l vs x).
+Proof.
+  induction l;intros;simpl in *. easy.
+  destruct a. simpl.
+  apply IHl.
+  specialize (vars_anti_vs_same (Rshift x) 0 vs (snd
+       (fst
+          (trans_exp vs 0 
+             (Rshift x) (fun _ : nat => (0, 0))))) (fun _ => (0,0))) as eq1.
+  apply eq1. easy. easy.
+  simpl.
+  apply IHl.
+  specialize (vars_anti_vs_same (Lshift x) 0 vs (snd
+       (fst
+          (trans_exp vs 0 
+             (Lshift x) (fun _ : nat => (0, 0))))) (fun _ => (0,0))) as eq1.
+  apply eq1. easy. easy.
+  simpl. apply IHl.
+  specialize (vars_anti_vs_same (Rev x) 0 vs (snd
+       (fst
+          (trans_exp vs 0 
+             (Rev x) (fun _ : nat => (0, 0))))) (fun _ => (0,0))) as eq1.
+  apply eq1. easy. easy.
+Qed.
+
+Lemma inter_neu_l_rev_same_1 : forall (l: list sexp) vs vs1 x, inter_neu_l_anti l vs x x = vs1 x ->
+       vars_anti_same vs -> inter_neu_l l vs1 x x = vs x.
+Proof.
+  induction l;intros. easy.
+  destruct a. simpl in *.
+  specialize (vars_anti_vs_same (Rshift x) 0 vs (snd
+       (fst
+          (trans_exp vs 0 
+             (Rshift x) (fun _ : nat => (0, 0))))) (fun _ => (0,0))) as eq1.
+  simpl in eq1. apply eq1 in H1 as eq2. clear eq1.
+  specialize (IHl (trans_rshift vs x) vs1 x).
+  unfold trans_lshift in *. rewrite IHl; try easy.
+  unfold trans_rshift. destruct (vs x) eqn:eq1. destruct p. destruct p.
+  bdestruct (x =? x).
+  bdestruct (x =? x).
+  rewrite shift_fun_twice_same_1.
+  rewrite ashift_fun_twice_same_1. easy.
+  unfold vars_anti_same in H1.
+  destruct (H1 x) as [X1 [X2 [X3 [X4 [X5 X6]]]]].
+  intros. specialize (X3 i).
+  unfold vsize,avmap in X3. rewrite eq1 in *. simpl in *. apply X3. easy.
+  lia. lia. easy.
+  simpl in *.
+  specialize (vars_anti_vs_same (Lshift x) 0 vs (snd
+       (fst
+          (trans_exp vs 0 
+             (Lshift x) (fun _ : nat => (0, 0))))) (fun _ => (0,0))) as eq1.
+  simpl in eq1. apply eq1 in H1 as eq2. clear eq1.
+  specialize (IHl (trans_lshift vs x) vs1 x).
+  unfold trans_rshift in *. rewrite IHl; try easy.
+  unfold trans_lshift. destruct (vs x) eqn:eq1. destruct p. destruct p.
+  bdestruct (x =? x).
+  bdestruct (x =? x).
+  rewrite shift_fun_twice_same.
+  rewrite ashift_fun_twice_same. easy.
+  unfold vars_anti_same in H1.
+  destruct (H1 x) as [X1 [X2 [X3 [X4 [X5 X6]]]]].
+  intros. specialize (X3 i).
+  unfold vsize,avmap in X3. rewrite eq1 in *. simpl in *. apply X3. easy.
+  lia. lia. easy.
+  simpl in *.
+  specialize (vars_anti_vs_same (Rev x) 0 vs (snd
+       (fst
+          (trans_exp vs 0 
+             (Rev x) (fun _ : nat => (0, 0))))) (fun _ => (0,0))) as eq1.
+  simpl in eq1. apply eq1 in H1 as eq2. clear eq1.
+  specialize (IHl (trans_rev vs x) vs1 x).
+  unfold trans_rev in *. rewrite IHl; try easy.
+  destruct (vs x) eqn:eq1. destruct p. destruct p.
+  bdestruct (x =? x).
+  bdestruct (x =? x).
+  rewrite fbrev_twice_same.
+  rewrite afbrev_twice_same. easy.
+  unfold vars_anti_same in H1.
+  destruct (H1 x) as [X1 [X2 [X3 [X4 [X5 X6]]]]].
+  intros. specialize (X3 i).
+  unfold vsize,avmap in X3. rewrite eq1 in *. simpl in *. apply X3. easy.
+  lia. lia. easy.
+Qed.
+
+
+Lemma inter_neu_l_var_same: forall l x vs vs1, vs x = vs1 x -> inter_neu_l l vs x x = inter_neu_l l vs1 x x.
+Proof.
+  induction l;intros;simpl in *. easy.
+  destruct a.
+  simpl.
+  unfold trans_lshift.
+  rewrite IHl with (vs1 := vs1);try easy.
+  destruct (inter_neu_l l vs1 x x) eqn:eq1. destruct p. destruct p.
+  bdestruct (x =? x). easy. lia.
+  simpl.
+  unfold trans_rshift.
+  rewrite IHl with (vs1 := vs1);try easy.
+  destruct (inter_neu_l l vs1 x x) eqn:eq1. destruct p. destruct p.
+  bdestruct (x =? x). easy. lia.
+  simpl.
+  unfold trans_rev.
+  rewrite IHl with (vs1 := vs1);try easy.
+  destruct (inter_neu_l l vs1 x x) eqn:eq1. destruct p. destruct p.
+  bdestruct (x =? x). easy. lia.
+Qed.
+
+Lemma inter_neu_l_assoc_1 : forall (l2 l1 l: list sexp) (vs vs1 vs2:vars) (x:var),
+       vars_anti_same vs -> vars_anti_same vs1 ->
+       l = l2++l1 -> inter_neu_l l vs x x = vs2 x -> inter_neu_l l2 vs1 x x = vs2 x
+         -> inter_neu_l l1 vs x x = vs1 x.
+Proof.
+  induction l2; intros; simpl in *.
+  subst. rewrite H4. rewrite <- H3. apply inter_neu_l_var_same with (vs1 := vs); try easy.
+  destruct l. inv H2. inv H2.
+  assert (vars_anti_same (inter_neu_l (l2 ++ l1) vs x)) as X1.
+  apply inter_neu_l_vars_anti_same; try easy.
+  assert (vars_anti_same (inter_neu_l l2 vs1 x)) as X2.
+  apply inter_neu_l_vars_anti_same; try easy.
+  simpl in *.
+  destruct a. simpl in *.
+  specialize (IHl2 l1 (l2++l1) vs vs1 (trans_rshift vs2 x) x).
+  rewrite IHl2; try easy.
+  unfold trans_rshift. rewrite <- H3.
+  unfold trans_lshift.
+  destruct (inter_neu_l (l2 ++ l1) vs x x) eqn:eq1.
+  destruct p. destruct p.
+  bdestruct (x =? x).
+  bdestruct (x =? x).
+  rewrite shift_fun_twice_same.
+  rewrite ashift_fun_twice_same. easy.
+  unfold vars_anti_same in X1.
+  destruct (X1 x) as [V1 [V2 [V3 [V4 [V5 V6]]]]].
+  intros. specialize (V3 i).
+  unfold vsize, avmap in *.
+  rewrite eq1 in *. simpl in *.
+  apply V3. easy. lia. lia.
+  unfold trans_rshift. rewrite <- H4.
+  unfold trans_lshift.
+  destruct (inter_neu_l l2 vs1 x x) eqn:eq1.
+  destruct p. destruct p.
+  bdestruct (x =? x).
+  bdestruct (x =? x).
+  rewrite shift_fun_twice_same.
+  rewrite ashift_fun_twice_same. easy.
+  unfold vars_anti_same in X2.
+  destruct (X2 x) as [V1 [V2 [V3 [V4 [V5 V6]]]]].
+  intros. specialize (V3 i).
+  unfold vsize, avmap in *.
+  rewrite eq1 in *. simpl in *.
+  apply V3. easy. lia. lia.
+  simpl in *.
+  specialize (IHl2 l1 (l2++l1) vs vs1 (trans_lshift vs2 x) x).
+  rewrite IHl2; try easy.
+  unfold trans_lshift. rewrite <- H3.
+  unfold trans_rshift.
+  destruct (inter_neu_l (l2 ++ l1) vs x x) eqn:eq1.
+  destruct p. destruct p.
+  bdestruct (x =? x).
+  bdestruct (x =? x).
+  rewrite shift_fun_twice_same_1.
+  rewrite ashift_fun_twice_same_1. easy.
+  unfold vars_anti_same in X1.
+  destruct (X1 x) as [V1 [V2 [V3 [V4 [V5 V6]]]]].
+  intros. specialize (V3 i).
+  unfold vsize, avmap in *.
+  rewrite eq1 in *. simpl in *.
+  apply V3. easy. lia. lia.
+  unfold trans_lshift. rewrite <- H4.
+  unfold trans_rshift.
+  destruct (inter_neu_l l2 vs1 x x) eqn:eq1.
+  destruct p. destruct p.
+  bdestruct (x =? x).
+  bdestruct (x =? x).
+  rewrite shift_fun_twice_same_1.
+  rewrite ashift_fun_twice_same_1. easy.
+  unfold vars_anti_same in X2.
+  destruct (X2 x) as [V1 [V2 [V3 [V4 [V5 V6]]]]].
+  intros. specialize (V3 i).
+  unfold vsize, avmap in *.
+  rewrite eq1 in *. simpl in *.
+  apply V3. easy. lia. lia.
+  simpl in *.
+  specialize (IHl2 l1 (l2++l1) vs vs1 (trans_rev vs2 x) x).
+  rewrite IHl2; try easy.
+  unfold trans_rev. rewrite <- H3.
+  unfold trans_rev.
+  destruct (inter_neu_l (l2 ++ l1) vs x x) eqn:eq1.
+  destruct p. destruct p.
+  bdestruct (x =? x).
+  bdestruct (x =? x).
+  rewrite fbrev_twice_same.
+  rewrite afbrev_twice_same. easy.
+  unfold vars_anti_same in X1.
+  destruct (X1 x) as [V1 [V2 [V3 [V4 [V5 V6]]]]].
+  intros. specialize (V3 i).
+  unfold vsize, avmap in *.
+  rewrite eq1 in *. simpl in *.
+  apply V3. easy. lia. lia.
+  unfold trans_rev. rewrite <- H4.
+  unfold trans_rev.
+  destruct (inter_neu_l l2 vs1 x x) eqn:eq1.
+  destruct p. destruct p.
+  bdestruct (x =? x).
+  bdestruct (x =? x).
+  rewrite fbrev_twice_same.
+  rewrite afbrev_twice_same. easy.
+  unfold vars_anti_same in X2.
+  destruct (X2 x) as [V1 [V2 [V3 [V4 [V5 V6]]]]].
+  intros. specialize (V3 i).
+  unfold vsize, avmap in *.
+  rewrite eq1 in *. simpl in *.
+  apply V3. easy. lia. lia.
+Qed.
+
+Lemma inter_neu_l_anti_assoc : forall (l2 l1 l: list sexp) (vs vs1 vs2:vars) (x:var),
+       vars_anti_same vs -> vars_anti_same vs1 -> vars_anti_same vs2 ->
+       l1 = l++l2 -> inter_neu_l l1 vs x x = vs1 x -> inter_neu_l_anti l vs1 x x = vs2 x
+         -> inter_neu_l l2 vs x x = vs2 x.
+Proof.
+  intros.
+  apply inter_neu_l_rev_same_1 in H5 ; try easy.
+  apply inter_neu_l_assoc_1 with (l2 := l) (l := l1) (vs2 := vs1); try easy.
+Qed.
+
+Lemma inter_neu_l_assoc_2 : forall (l2 l1 l: list sexp) (vs vs1 vs2:vars) (x:var),
+       vars_anti_same vs -> vars_anti_same vs2 ->
+       l = l2++l1 -> inter_neu_l l vs x x = vs2 x -> inter_neu_l l1 vs x x = vs1 x
+         -> inter_neu_l l2 vs1 x x = vs2 x.
+Proof.
+  induction l2; intros; simpl in *.
+  subst. rewrite <- H4. rewrite H3. easy.
+  destruct l. inv H2. inv H2.
+  assert (vars_anti_same (inter_neu_l (l2 ++ l1) vs x)) as X1.
+  apply inter_neu_l_vars_anti_same; try easy.
+  assert (vars_anti_same (inter_neu_l l1 vs x)) as X2.
+  apply inter_neu_l_vars_anti_same; try easy.
+  simpl in *.
+  destruct a. simpl in *.
+  specialize (IHl2 l1 (l2++l1) vs vs1 (trans_rshift vs2 x) x).
+  unfold trans_lshift in *.
+  rewrite IHl2; try easy.
+  unfold trans_rshift. 
+  destruct (vs2 x) eqn:eq1. destruct p. destruct p.
+  bdestruct (x =? x).
+  bdestruct (x =? x).
+  rewrite shift_fun_twice_same_1.
+  rewrite ashift_fun_twice_same_1. easy.
+  unfold vars_anti_same in H1.
+  destruct (H1 x) as [V1 [V2 [V3 [V4 [V5 V6]]]]].
+  intros. specialize (V3 i).
+  unfold vsize, avmap in *.
+  rewrite eq1 in *. simpl in *.
+  apply V3. easy. lia. lia.
+  Check vars_anti_vs_same.
+  specialize (vars_anti_vs_same (Rshift x) 0 vs2 
+   (snd (fst (trans_exp vs2 0 (Rshift x) (fun _ => (0,0))))) (fun _ => (0,0))) as X3.
+  simpl in X3. apply X3. easy. easy.
+  unfold trans_rshift. rewrite <- H3.
+  destruct (inter_neu_l (l2 ++ l1) vs x x) eqn:eq1.
+  destruct p. destruct p.
+  bdestruct (x =? x).
+  bdestruct (x =? x).
+  rewrite shift_fun_twice_same.
+  rewrite ashift_fun_twice_same. easy.
+  unfold vars_anti_same in X1.
+  destruct (X1 x) as [V1 [V2 [V3 [V4 [V5 V6]]]]].
+  intros. specialize (V3 i).
+  unfold vsize, avmap in *.
+  rewrite eq1 in *. simpl in *.
+  apply V3. easy. lia. lia.
+  simpl in *.
+  specialize (IHl2 l1 (l2++l1) vs vs1 (trans_lshift vs2 x) x).
+  unfold trans_rshift in *.
+  rewrite IHl2; try easy.
+  unfold trans_lshift. 
+  destruct (vs2 x) eqn:eq1. destruct p. destruct p.
+  bdestruct (x =? x).
+  bdestruct (x =? x).
+  rewrite shift_fun_twice_same.
+  rewrite ashift_fun_twice_same. easy.
+  unfold vars_anti_same in H1.
+  destruct (H1 x) as [V1 [V2 [V3 [V4 [V5 V6]]]]].
+  intros. specialize (V3 i).
+  unfold vsize, avmap in *.
+  rewrite eq1 in *. simpl in *.
+  apply V3. easy. lia. lia.
+  Check vars_anti_vs_same.
+  specialize (vars_anti_vs_same (Lshift x) 0 vs2 
+   (snd (fst (trans_exp vs2 0 (Lshift x) (fun _ => (0,0))))) (fun _ => (0,0))) as X3.
+  simpl in X3. apply X3. easy. easy.
+  unfold trans_lshift. rewrite <- H3.
+  destruct (inter_neu_l (l2 ++ l1) vs x x) eqn:eq1.
+  destruct p. destruct p.
+  bdestruct (x =? x).
+  bdestruct (x =? x).
+  rewrite shift_fun_twice_same_1.
+  rewrite ashift_fun_twice_same_1. easy.
+  unfold vars_anti_same in X1.
+  destruct (X1 x) as [V1 [V2 [V3 [V4 [V5 V6]]]]].
+  intros. specialize (V3 i).
+  unfold vsize, avmap in *.
+  rewrite eq1 in *. simpl in *.
+  apply V3. easy. lia. lia.
+  simpl in *.
+  specialize (IHl2 l1 (l2++l1) vs vs1 (trans_rev vs2 x) x).
+  unfold trans_rev in *.
+  rewrite IHl2; try easy.
+  destruct (vs2 x) eqn:eq1. destruct p. destruct p.
+  bdestruct (x =? x).
+  bdestruct (x =? x).
+  rewrite fbrev_twice_same.
+  rewrite afbrev_twice_same. easy.
+  unfold vars_anti_same in H1.
+  destruct (H1 x) as [V1 [V2 [V3 [V4 [V5 V6]]]]].
+  intros. specialize (V3 i).
+  unfold vsize, avmap in *.
+  rewrite eq1 in *. simpl in *.
+  apply V3. easy. lia. lia.
+  Check vars_anti_vs_same.
+  specialize (vars_anti_vs_same (Rev x) 0 vs2 
+   (snd (fst (trans_exp vs2 0 (Rev x) (fun _ => (0,0))))) (fun _ => (0,0))) as X3.
+  simpl in X3. apply X3. easy. easy.
+  rewrite <- H3.
+  destruct (inter_neu_l (l2 ++ l1) vs x x) eqn:eq1.
+  destruct p. destruct p.
+  bdestruct (x =? x).
+  bdestruct (x =? x).
+  rewrite fbrev_twice_same.
+  rewrite afbrev_twice_same. easy.
+  unfold vars_anti_same in X1.
+  destruct (X1 x) as [V1 [V2 [V3 [V4 [V5 V6]]]]].
+  intros. specialize (V3 i).
+  unfold vsize, avmap in *.
+  rewrite eq1 in *. simpl in *.
+  apply V3. easy. lia. lia.
+Qed.
+
+Lemma inter_neu_l_vs_same: forall l vs vs' x, vs x = vs' x -> inter_neu_l l vs x x = inter_neu_l l vs' x x.
+Proof.
+  induction l; intros; simpl in *. easy.
+  destruct a. simpl.
+  unfold trans_lshift.
+  rewrite IHl with (vs' := vs'); try easy. 
+  destruct (inter_neu_l l vs' x x) eqn:eq1. destruct p. destruct p.
+  bdestruct (x =? x). easy. lia.
+  simpl.
+  unfold trans_rshift.
+  rewrite IHl with (vs' := vs'); try easy. 
+  destruct (inter_neu_l l vs' x x) eqn:eq1. destruct p. destruct p.
+  bdestruct (x =? x). easy. lia.
+  simpl.
+  unfold trans_rev.
+  rewrite IHl with (vs' := vs'); try easy. 
+  destruct (inter_neu_l l vs' x x) eqn:eq1. destruct p. destruct p.
+  bdestruct (x =? x). easy. lia.
+Qed.
+
+
+Lemma neu_l_trans_state : forall e l l' x (vs:vars) (dim:nat) (avs : nat -> posi),
+      exp_neu_l x l e l' -> vars_anti_same vs ->
+      exp_neu_trans_prop x l l' vs (snd (fst (trans_exp vs dim e avs))).
+Proof.
+  induction e; intros; simpl in *.
+  inv H0. unfold exp_neu_trans_prop in *.
+  bdestruct (length l' <=? length l').
+  intros.
+  apply get_cut_n_list_same_2 in H2. rewrite H2 in *. inv H3.
+  simpl. easy. lia.
+  inv H0. unfold exp_neu_trans_prop in *.
+  bdestruct (length l' <=? length l').
+  intros.
+  apply get_cut_n_list_same_2 in H2. rewrite H2 in *. inv H3.
+  simpl. easy. lia.
+  inv H0. unfold exp_neu_trans_prop in *.
+  destruct (trans_exp vs dim e avs) eqn:eq1. destruct p0.
+  bdestruct (length l' <=? length l').
+  intros.
+  apply get_cut_n_list_same_2 in H2. rewrite H2 in *. inv H3.
+  simpl. easy. lia.
+  inv H0. unfold exp_neu_trans_prop in *.
+  bdestruct (length l' <=? length l').
+  intros.
+  apply get_cut_n_list_same_2 in H2. rewrite H2 in *. inv H3.
+  simpl. easy. lia.
+  inv H0. unfold exp_neu_trans_prop in *.
+  bdestruct (length l' <=? length l').
+  intros.
+  apply get_cut_n_list_same_2 in H2. rewrite H2 in *. inv H3.
+  simpl. easy. lia.
+  inv H0. unfold exp_neu_trans_prop in *.
+  bdestruct (length l' <=? length l').
+  intros.
+  apply get_cut_n_list_same_2 in H2. rewrite H2 in *. inv H3.
+  simpl. easy. lia.
+  inv H0. unfold exp_neu_trans_prop in *.
+  bdestruct (length l' <=? length l').
+  intros.
+  apply get_cut_n_list_same_2 in H2. rewrite H2 in *. inv H3.
+  simpl. easy. lia.
+  inv H0. unfold exp_neu_trans_prop in *.
+  bdestruct (length l' <=? length l').
+  intros.
+  apply get_cut_n_list_same_2 in H2. rewrite H2 in *. inv H3.
+  simpl. easy. lia.
+  inv H0. unfold exp_neu_trans_prop in *.
+  bdestruct (length (Rs :: l') <=? length l'). simpl in *. lia.
+  intros.
+  apply get_cut_n_list_1 in H2. subst. simpl in *. inv H3.
+  simpl. easy.
+  unfold exp_neu_trans_prop in *.
+  bdestruct (length l <=? length (Ls :: l)).
+  intros.
+  apply get_cut_n_list_1 in H2. subst. simpl in *. inv H3.
+  simpl. easy. simpl in *. lia.
+  unfold exp_neu_trans_prop in *.
+  bdestruct (length l' <=? length l').
+  intros.
+  apply get_cut_n_list_same_2 in H2. rewrite H2 in *. inv H3.
+  simpl.
+  unfold trans_lshift.
+  destruct (vs x) eqn:eq1. destruct p. destruct p.
+  bdestruct (x0 =? x). lia. easy. lia.
+  inv H0. unfold exp_neu_trans_prop in *.
+  bdestruct (length (Ls :: l') <=? length l'). simpl in *. lia.
+  intros.
+  apply get_cut_n_list_1 in H2. subst. simpl in *. inv H3.
+  simpl. easy.
+  unfold exp_neu_trans_prop in *.
+  bdestruct (length l <=? length (Rs :: l)).
+  intros.
+  apply get_cut_n_list_1 in H2. subst. simpl in *. inv H3.
+  simpl. easy. simpl in *. lia.
+  unfold exp_neu_trans_prop in *.
+  bdestruct (length l' <=? length l').
+  intros.
+  apply get_cut_n_list_same_2 in H2. rewrite H2 in *. inv H3.
+  simpl.
+  unfold trans_rshift.
+  destruct (vs x) eqn:eq1. destruct p. destruct p.
+  bdestruct (x0 =? x). lia. easy. lia.
+  inv H0. unfold exp_neu_trans_prop in *.
+  bdestruct (length (Re :: l') <=? length l'). simpl in *. lia.
+  intros.
+  apply get_cut_n_list_1 in H2. subst. simpl in *. inv H3.
+  simpl. easy.
+  unfold exp_neu_trans_prop in *.
+  bdestruct (length l <=? length (Re :: l)).
+  intros.
+  apply get_cut_n_list_1 in H2. subst. simpl in *. inv H3.
+  simpl. easy. simpl in *. lia.
+  unfold exp_neu_trans_prop in *.
+  bdestruct (length l' <=? length l').
+  intros.
+  apply get_cut_n_list_same_2 in H2. rewrite H2 in *. inv H3.
+  simpl.
+  unfold trans_rev.
+  destruct (vs x) eqn:eq1. destruct p. destruct p.
+  bdestruct (x0 =? x). lia. easy. lia.
+  inv H0. unfold exp_neu_trans_prop in *.
+  bdestruct (length l' <=? length l').
+  intros.
+  apply get_cut_n_list_same_2 in H2. rewrite H2 in *. inv H3.
+  simpl. easy. lia.
+  inv H0. unfold exp_neu_trans_prop in *.
+  bdestruct (length l' <=? length l').
+  intros.
+  apply get_cut_n_list_same_2 in H2. rewrite H2 in *. inv H3.
+  simpl. easy. lia.
+  inv H0. unfold exp_neu_trans_prop in *.
+  bdestruct (length l' <=? length l').
+  intros.
+  apply get_cut_n_list_same_2 in H2. rewrite H2 in *. inv H3.
+  simpl. easy. lia.
+  destruct (trans_exp vs dim e1 avs) eqn:eq1. destruct p.
+  destruct (trans_exp v dim e2 p0) eqn:eq2. destruct p.
+  inv H0.
+  specialize (IHe1 l l'0 x vs dim avs H5 H1).
+  rewrite eq1 in *.
+  assert (vars_anti_same v) as V1.
+  specialize (vars_anti_vs_same e1 dim vs v avs) as X1.
+  apply X1. rewrite eq1. easy. easy.
+  assert (vars_anti_same v0) as V2.
+  specialize (vars_anti_vs_same e2 dim v v0 p0) as X1.
+  apply X1. rewrite eq2. easy. easy.
+  specialize (IHe2 l'0 l' x v dim p0 H7 V1).
+  rewrite eq2 in *. simpl in *.
+  unfold exp_neu_trans_prop in *.
+  bdestruct (length l <=? length l'0).
+  bdestruct (length l'0 <=? length l').
+  bdestruct (length l <=? length l'). intros.
+  apply exp_neu_sub_keep in H5 as X1.
+  unfold exp_neu_sub_prop in X1.
+  destruct X1. destruct H8.
+  apply cut_get_l_exists in H8 as X1.
+  destruct X1.
+  apply get_cut_n_list_n in H4 as X1.
+  apply get_cut_n_list_n in H8 as X2.
+  specialize (get_cut_n_list_same x0 l'0 l x1 H8 H9) as X3.
+  specialize (IHe1 x0 x1 H8 H9).
+  apply exp_neu_sub_keep in H7 as X4.
+  unfold exp_neu_sub_prop in X4.
+  destruct X4. destruct H10.
+  apply cut_get_l_exists in H10 as X4.
+  destruct X4.
+  apply get_cut_n_list_n in H10 as X4.
+  specialize (get_cut_n_list_same x2 l' l'0 x3 H10 H11) as X5.
+  specialize (IHe2 x2 x3 H10 H11).
+  rewrite IHe2.
+  specialize (get_cut_n_list_same n l' l l1 H4 H6) as X6.
+  rewrite <- X3 in X5.
+  rewrite <- X5 in X6.
+  rewrite app_assoc in X6.
+  apply app_inv_tail in X6.
+  Check inter_neu_l_assoc.
+  specialize (inter_neu_l_assoc x3 x1 l1 vs v (inter_neu_l x3 v x) x X6) as X7.
+  rewrite X7; try easy.
+  apply get_cut_n_list_n in H10 as X4.
+  assert (x2 = 0) by lia.
+  rewrite H11 in *.
+  apply cut_get_l_exists in H10 as X5. destruct X5.
+  specialize (get_cut_n_list_same 0 l'0 l' x3 H10 H12) as X6.
+  assert (l'0 = l').
+  rewrite cut_n_list_0 in H10. clear X4. inv H10. easy. rewrite H13 in *. clear H13.
+  apply get_cut_n_list_same_2 in H10 as X7.
+  specialize (IHe2 0 ([]) H10 X7).
+  simpl in *. rewrite IHe2 in *. 
+  rewrite <- X1 in *. rewrite X2 in *. rewrite H6 in *. rewrite IHe1. inv H9. easy.
+  apply get_cut_n_list_n in H8 as X1.
+  assert (x0 = 0) by lia. rewrite H9 in *. clear H9 X1.
+  assert (l = l'0). rewrite cut_n_list_0 in H8. inv H8. easy.
+  rewrite H9 in *. clear H9.
+  apply get_cut_n_list_same_2 in H8 as X1.
+  specialize (IHe1 0 ([]) H8 X1).
+  simpl in *.
+  rewrite inter_neu_l_vs_same with (vs' := v); try easy.
+  apply IHe2 with (n := n); try easy. lia.
+  bdestruct (length l <=? length l'). intros.
+  apply exp_neu_sub_keep in H5.
+  apply exp_neu_sub_keep in H7.
+  unfold exp_neu_sub_prop in *. destruct H5. destruct H7.
+  destruct H5. destruct H7.
+  apply cut_l_length_le in H7. lia.
+  apply cut_get_l_exists in H5 as X1.
+  apply cut_get_l_exists in H7 as X2.
+  destruct X1. destruct X2.
+  specialize (IHe1 x0 x2 H5 H8).
+  specialize (IHe2 x1 x3 H7 H9).
+  Check get_cut_n_list_same.
+  specialize (get_cut_n_list_same x0 l'0 l x2 H5 H8) as X1.
+  specialize (get_cut_n_list_same x1 l'0 l' x3 H7 H9) as X2.
+  specialize (get_cut_n_list_same n l' l l1 H4 H6) as X3.
+  rewrite <- X3 in X2.
+  rewrite <- X2 in X1.
+  rewrite app_assoc in X1.
+  apply app_inv_tail in X1.
+  rewrite inter_neu_l_anti_assoc with (l1 := x2) (l := x3) (l2 := l1) (vs1 := v) (vs2 := v0); try easy.
+  apply cut_l_length_le in H5. lia.
+  intros. 
+  apply exp_neu_sub_keep in H5.
+  apply exp_neu_sub_keep in H7.
+  unfold exp_neu_sub_prop in *. destruct H5. destruct H7.
+  destruct H5. destruct H7.
+  apply cut_l_length_le in H7. lia.
+  apply cut_get_l_exists in H5 as X1.
+  apply cut_get_l_exists in H7 as X2.
+  destruct X1. destruct X2.
+  specialize (IHe1 x0 x2 H5 H8).
+  specialize (IHe2 x1 x3 H7 H9).
+  specialize (get_cut_n_list_same x0 l'0 l x2 H5 H8) as X1.
+  specialize (get_cut_n_list_same x1 l'0 l' x3 H7 H9) as X2.
+  specialize (get_cut_n_list_same n l l' l1 H4 H6) as X3.
+  rewrite <- X3 in X1.
+  rewrite <- X2 in X1.
+  rewrite app_assoc in X1.
+  apply app_inv_tail in X1.
+  Check inter_neu_l_anti_assoc.
+  symmetry.
+  apply inter_neu_l_rev_same; try easy.
+  symmetry in IHe2.
+  apply inter_neu_l_rev_same_1 in IHe2 ; try easy.
+  symmetry in IHe1. symmetry in X1.
+  Check inter_neu_l_assoc_1.
+  apply inter_neu_l_assoc_1 with (l2 := x2) (l := x3) (vs2 := v); try easy.
+  apply cut_l_length_le in H5 as X1.
+  assert (length l = length l'0) by lia. clear X1.
+  destruct H7.
+  apply cut_l_length_le in H7 as X1. lia.
+  apply get_cut_n_list_n in H5 as X2.
+  assert (x0 = 0) by lia. rewrite H9 in *. clear H9. clear X2.
+  apply cut_get_l_exists in H5 as X1.
+  apply cut_get_l_exists in H7 as X2.
+  destruct X1. destruct X2.
+  assert (l = l'0).
+  rewrite cut_n_list_0 in H5. inv H5. easy. rewrite H11 in *. clear H11.
+  specialize (IHe1 0 x2 H5 H9).
+  specialize (IHe2 x1 x3 H7 H10).
+  specialize (get_cut_n_list_same 0 l'0 l'0 x2 H5 H9) as X1.
+  assert (x2 = ([])).
+  assert (x2 ++ l'0 = ([])++l'0). rewrite app_nil_l. easy.
+  apply app_inv_tail in H11. easy. rewrite H11 in *.
+  simpl in IHe1.
+  apply get_cut_n_list_n in H7. apply get_cut_n_list_n in H4. rewrite <- H7 in H4. 
+  rewrite H4 in *. rewrite H10 in H6.
+  assert (x3 = l1). inv H6. easy.
+  rewrite H12 in *.
+  symmetry in IHe2.
+  apply inter_neu_l_rev_same_1 in IHe2; try easy.
+  rewrite IHe1 in *.
+  apply inter_neu_l_rev_same in IHe2; try easy.
+  bdestruct (length l'0 <=? length l').
+  bdestruct (length l <=? length l'). intros.
+  apply exp_neu_sub_keep in H5.
+  apply exp_neu_sub_keep in H7.
+  unfold exp_neu_sub_prop in *. destruct H5. destruct H7.
+  destruct H5.
+  apply cut_l_length_le in H5. lia.
+  destruct H7.
+  apply cut_get_l_exists in H5 as X1.
+  apply cut_get_l_exists in H7 as X2.
+  destruct X1. destruct X2.
+  specialize (IHe1 x0 x2 H5 H8).
+  specialize (IHe2 x1 x3 H7 H9).
+  Check get_cut_n_list_same.
+  specialize (get_cut_n_list_same x0 l l'0 x2 H5 H8) as X1.
+  specialize (get_cut_n_list_same x1 l' l'0 x3 H7 H9) as X2.
+  specialize (get_cut_n_list_same n l' l l1 H4 H6) as X3.
+  rewrite <- X1 in X3.
+  rewrite <- X2 in X3.
+  rewrite app_assoc in X3.
+  apply app_inv_tail in X3.
+  symmetry in IHe1.
+  apply inter_neu_l_rev_same_1 in IHe1; try easy.
+  symmetry.
+  apply inter_neu_l_assoc_2 with (l1 := x2) (l := x3) (vs := v); try easy.
+  apply cut_l_length_le in H7 as X1. lia.
+  intros.
+  apply exp_neu_sub_keep in H5.
+  apply exp_neu_sub_keep in H7.
+  unfold exp_neu_sub_prop in *. destruct H5. destruct H7.
+  destruct H5.
+  apply cut_l_length_le in H5. lia.
+  destruct H7.
+  apply cut_get_l_exists in H5 as X1.
+  apply cut_get_l_exists in H7 as X2.
+  destruct X1. destruct X2.
+  specialize (IHe1 x0 x2 H5 H8).
+  specialize (IHe2 x1 x3 H7 H9).
+  Check get_cut_n_list_same.
+  specialize (get_cut_n_list_same x0 l l'0 x2 H5 H8) as X1.
+  specialize (get_cut_n_list_same x1 l' l'0 x3 H7 H9) as X2.
+  specialize (get_cut_n_list_same n l l' l1 H4 H6) as X3.
+  rewrite <- X2 in X3.
+  rewrite <- X1 in X3.
+  rewrite app_assoc in X3.
+  apply app_inv_tail in X3.
+  symmetry in IHe1.
+  apply inter_neu_l_rev_same_1 in IHe1; try easy.
+  symmetry.
+  apply inter_neu_l_rev_same; try easy.
+  Check inter_neu_l_assoc_2.
+  apply inter_neu_l_assoc_2 with (l1 := x3) (l := x2) (vs := v); try easy.
+  apply cut_l_length_le in H7 as X1.
+  assert (length l' = length l'0) by lia.
+  apply get_cut_n_list_n in H7 as X2.
+  rewrite H8 in *. assert (x1 = 0) by lia.
+  rewrite H9 in *. clear H9.
+  assert (l'0 = l').
+  rewrite cut_n_list_0 in H7. inv H7. easy.
+  rewrite H9 in *. clear H9.
+  apply cut_get_l_exists in H5 as X3.
+  apply cut_get_l_exists in H7 as X4.
+  destruct X3. destruct X4.
+  assert (x3 = []).
+  Check get_cut_n_list_same.
+  specialize (get_cut_n_list_same 0 l' l' x3 H7 H10) as X5.
+  assert (x3 ++ l' = ([])++l').
+  rewrite  app_nil_l. easy.
+  apply app_inv_tail in H11. easy.
+  rewrite H11 in *. clear H11.
+  specialize (IHe1 x0 x2 H5 H9).
+  specialize (IHe2 0 ([]) H7 H10).
+  simpl in IHe2.
+  rewrite IHe2 in *.
+  assert (x0 = n).
+  apply get_cut_n_list_n in H5.
+  apply get_cut_n_list_n in H4. rewrite <- H4 in *. easy.
+  rewrite H11 in *.
+  rewrite H9 in *. inv H6. easy.
+  bdestruct (length l <=? length l'). lia.
+  intros.
+  symmetry.
+  apply inter_neu_l_rev_same; try easy.
+  apply exp_neu_sub_keep in H5.
+  apply exp_neu_sub_keep in H7.
+  unfold exp_neu_sub_prop in *. destruct H5. destruct H7.
+  destruct H5.
+  apply cut_l_length_le in H5. lia.
+  destruct H7.
+  apply cut_l_length_le in H7. lia.
+  apply cut_get_l_exists in H5 as X1.
+  apply cut_get_l_exists in H7 as X2.
+  destruct X1. destruct X2.
+  specialize (IHe1 x0 x2 H5 H8).
+  specialize (IHe2 x1 x3 H7 H9).
+  Check get_cut_n_list_same.
+  specialize (get_cut_n_list_same x0 l l'0 x2 H5 H8) as X1.
+  specialize (get_cut_n_list_same x1 l'0 l' x3 H7 H9) as X2.
+  specialize (get_cut_n_list_same n l l' l1 H4 H6) as X3.
+  rewrite <- X2 in X1.
+  rewrite <- X3 in X1.
+  rewrite app_assoc in X1.
+  apply app_inv_tail in X1.
+  symmetry in IHe1.
+  apply inter_neu_l_rev_same_1 in IHe1; try easy.
+  symmetry in IHe2.
+  apply inter_neu_l_rev_same_1 in IHe2; try easy.
+  Check inter_neu_l_assoc.
+  apply inter_neu_l_assoc with (l2 := x2) (l1 := x3) (vs1 := v); try easy.
+Qed.
 
 
 Lemma in_list_x : forall (l:list nat) x, In x l \/ ~ In x l.
@@ -6422,25 +7596,159 @@ Proof.
   rewrite eq2 in H1. simpl in H1. rewrite IHe1 in H1. easy.
 Qed.
 
-Lemma neu_trans_state : forall e vs dim avs, exp_neu (get_vars e) e -> snd (fst (trans_exp vs dim e avs)) = vs.
+
+Lemma neu_trans_state : forall e vs dim avs, exp_neu (get_vars e) e
+    -> vars_anti_same vs -> (snd (fst (trans_exp vs dim e avs))) = vs.
 Proof.
   intros.
-  unfold exp_neu in H0.
-  apply functional_extensionality. intros.
-  specialize (in_list_x (get_vars e) x) as eq1.
-  destruct eq1.
-  apply H0 in H1.
-  apply neu_l_trans_state with (vs := vs) (dim := dim) (avs:=avs) in H1. easy.
-  specialize (trans_finnite_no_in e vs (get_vars e) dim avs) as eq1.
-  assert (forall u : var, In u (get_vars e) -> In u (get_vars e)).
-  intros. easy.
-  specialize (eq1 H2 x H1). easy.
+  apply functional_extensionality; intro.
+  assert (In x (get_vars e) \/ ~ In x (get_vars e)).
+  destruct (@in_dec var Nat.eq_dec x (get_vars e)). left. easy. right. easy.
+  destruct H2.
+  unfold exp_neu in *. specialize (H0 x). apply H0 in H2.
+  specialize (neu_l_trans_state e ([]) ([]) x vs dim avs H2 H1) as eq1.
+  unfold exp_neu_trans_prop in *. simpl in *.
+  specialize (eq1 0 ([])).
+  assert (@cut_n_list sexp 0 ([]) = Some ([])).
+  simpl. easy. apply eq1 in H3. rewrite H3. simpl. easy. easy.
+  rewrite trans_finnite_no_in with (avars := get_vars e); try easy.
 Qed.
 
-Lemma neu_trans_state_avs : forall e vs dim avs, exp_neu (get_vars e) e -> snd  (trans_exp vs dim e avs) = avs.
+Lemma avs_out_1 : forall e vs dim avs,
+      (forall i, dim <= i -> snd (trans_exp vs dim e avs) i = avs i).
+Proof.
+  induction e; intros; try easy.
+  simpl in *.
+  destruct (trans_exp vs dim e avs) eqn:eq1. destruct p0.  simpl. easy.
+  simpl in *.
+  unfold lshift_avs.
+  bdestruct (i <? dim). lia.
+  simpl. easy.
+  simpl in *.
+  unfold rshift_avs.
+  bdestruct (i <? dim). lia.
+  simpl. easy.
+  simpl in *.
+  unfold rev_avs.
+  bdestruct (i <? dim). lia.
+  simpl. easy.
+  simpl in *.
+  destruct (trans_exp vs dim e1 avs) eqn:eq1. destruct p.
+  destruct (trans_exp v dim e2 p0) eqn:eq2. destruct p.
+  simpl in *.
+  specialize (IHe1 vs dim avs i).
+  apply IHe1 in H0 as X1.
+  rewrite eq1 in *. simpl in *. rewrite <- X1.
+  specialize (IHe2 v dim p0 i).
+  apply IHe2 in H0 as X2.
+  rewrite eq2 in *. simpl in *. easy.
+Qed.
+
+Lemma avs_prop_trans_fst_same : forall e vs dim avs, avs_prop vs avs dim ->
+        vars_anti_same vs -> vars_sparse vs ->
+         (forall i, i < dim -> fst ((snd  (trans_exp vs dim e avs)) i) = fst (avs i)).
+Proof.
+  induction e; intros; try easy.
+  simpl in *. destruct (trans_exp vs dim e avs) eqn:eq1. destruct p0.
+  simpl in *. easy.
+  simpl.
+  unfold lshift_avs.
+  bdestruct (i <? dim).
+  bdestruct ((start vs x <=? i)).
+  bdestruct ((i - start vs x <? vsize vs x)).
+  simpl.
+  bdestruct (fst (avs i) =? x). easy.
+  Check var_not_over_lap_1.
+  specialize (var_not_over_lap_1 x (avs i) vs H2 H1) as eq1.
+  apply eq1 in H7.
+  destruct H7.
+  rewrite vs_avs_bij_r with (dim := dim) in H7; try easy. lia.
+  rewrite vs_avs_bij_r with (dim := dim) in H7; try easy. lia.
+  apply vs_avs_size with (dim := dim) ; try easy.
+  1-3:simpl; easy.
+  simpl.
+  unfold rshift_avs.
+  bdestruct (i <? dim).
+  bdestruct ((start vs x <=? i)).
+  bdestruct ((i - start vs x <? vsize vs x)).
+  simpl.
+  bdestruct (fst (avs i) =? x). easy.
+  Check var_not_over_lap_1.
+  specialize (var_not_over_lap_1 x (avs i) vs H2 H1) as eq1.
+  apply eq1 in H7.
+  destruct H7.
+  rewrite vs_avs_bij_r with (dim := dim) in H7; try easy. lia.
+  rewrite vs_avs_bij_r with (dim := dim) in H7; try easy. lia.
+  apply vs_avs_size with (dim := dim) ; try easy.
+  1-3:simpl; easy.
+  simpl.
+  unfold rev_avs.
+  bdestruct (i <? dim).
+  bdestruct ((start vs x <=? i)).
+  bdestruct ((i - start vs x <? vsize vs x)).
+  simpl.
+  bdestruct (fst (avs i) =? x). easy.
+  Check var_not_over_lap_1.
+  specialize (var_not_over_lap_1 x (avs i) vs H2 H1) as eq1.
+  apply eq1 in H7.
+  destruct H7.
+  rewrite vs_avs_bij_r with (dim := dim) in H7; try easy. lia.
+  rewrite vs_avs_bij_r with (dim := dim) in H7; try easy. lia.
+  apply vs_avs_size with (dim := dim) ; try easy.
+  1-3:simpl; easy.
+  simpl in *.
+  destruct (trans_exp vs dim e1 avs) eqn:eq1. destruct p.
+  destruct (trans_exp v dim e2 p0) eqn:eq2. destruct p.
+  simpl in *.
+  specialize (IHe1 vs dim avs H0 H1 H2 i H3).
+  rewrite eq1 in IHe1. simpl in *.
+  rewrite <- IHe1.
+  Check avs_prop_vs_same.
+  specialize (avs_prop_vs_same e1 dim vs v avs p0) as X1.
+  rewrite eq1 in *. simpl in *.
+  apply X1 in H1 as X2 ; try easy.
+  Check vars_sparse_vs_same.
+  specialize (vars_sparse_vs_same e1 dim vs v avs) as X3.
+  rewrite eq1 in *. simpl in X3.
+  assert (v = v) by easy. apply X3 in H4. clear X3.
+  specialize (vars_anti_vs_same e1 dim vs v avs) as X3.
+  rewrite eq1 in *.
+  assert (v = v) by easy. apply X3 in H5. clear X3.
+  specialize (IHe2 v dim p0 X2 H5 H4 i H3).
+  rewrite eq2 in IHe2. simpl in *. easy.
+  easy. easy.
+Qed.
+
+Lemma neu_trans_state_avs : forall e vs dim avs, avs_prop vs avs dim 
+         -> vars_anti_same vs -> vars_sparse vs -> exp_com_WF vs dim ->
+           exp_neu (get_vars e) e -> snd  (trans_exp vs dim e avs) = avs.
 Proof.
   intros.
-Admitted.
+  specialize (neu_trans_state e vs dim avs H4 H1) as eq1.
+  apply functional_extensionality; intro.
+  bdestruct (x <? dim).
+  remember (snd (fst (trans_exp vs dim e avs))) as vs'.
+  remember (snd (trans_exp vs dim e avs)) as avs'.
+  Check avs_prop_vs_same.
+  specialize (avs_prop_vs_same e dim vs vs' avs avs' Heqvs' Heqavs' H1 H2 H0) as eq2.
+  rewrite eq1 in *.
+  assert (exists i, x = find_pos vs i).
+  exists (avs x).
+  rewrite vs_avs_bij_r with (dim := dim); try easy.
+  destruct H6. rewrite H6.
+  Check avs_prop_trans_fst_same.
+  assert (fst (avs' x) = fst (avs x)).
+  rewrite Heqavs'.
+  apply avs_prop_trans_fst_same; try easy.
+  unfold avs_prop in *.
+  specialize (H0 x H5). specialize (eq2 x H5).
+  destruct H0 as [X1 [X2 X3]].
+  destruct eq2 as [V1 [V2 V3]].
+  rewrite H7 in *.
+  rewrite X3 in V3. rewrite <- H6 in *.
+  destruct (avs' x). destruct (avs x). simpl in *. subst. easy.
+  rewrite avs_out_1. easy. lia.
+Qed.
 
 
 (*
